1✅
A={2,3,5} B={2,4,6}  C={1,2,3,4}  
P(A)=1/2 P(B)=1/2  P(C)=2/3
P(A)P(C)=1/2\*2/3=1/3=P(A$\cap$C) => the are independent
P(A|B)=P(A$\cap$B)/P(B)=1/6  / 1/2 = 1/3

---
2✅
You have a partition $\Omega\ =\ \left\{a,\ b\ ,\ c\ ,\ d\ ,\ e,\ f\right\}$
a) $A_{1}\cup\ A_{2}\ \cup\ A_{3}=\left\{a\right\}\ \ P\left(a\right)=\frac{1}{27}$
$P\left(A_{1}\right)=P\left(A_{2}\right)=P\left(A_{3}\right)=\frac{1}{3}$
$P\left(A_{1}\right)P\left(A_{2}\right)P\left(A_{3}\right)=P\left(A_{1}\cup\ A_{2}\ \cup\ A_{3}\right)=\frac{1}{27}$
b) just take $P(A_1 \cup A_2)\neq P(A_1)P(A_2)$

---
3✅
A: the probability that the first loto cards matches one of the 4 drawn numbers
B: the probability that the second ...
$$P(A)=\frac{85\binom{5}{4}}{\binom{90}{5}}=P(B)$$
They are independent events.
$P(A\cup B)=P(A)+P(B)-P(A\cap B)=2P(A)+P(A)^2$ 

---
4✅
S1: the fist proxy landed in one of the servers
S2: the second proxy landed not in the server that the first proxy landed
S3: the third proxy landed not in the server that the first and second proxy landed
S4: ....
We use the multiplication rule
P(S1 S2 S3 S4) = P(S1)P(S2|S1)P(S3|S1S2)P(S4|S3S2S1)=1\*5/6\*4/6\*3/6 = 5/18

---
5✅
P(A$\cup$B)=P(A)+P(B)-P(A$\cap$B)=1 
P(A|B)=P(A$\cap$B)/P(B) = 0.2
P(B|A)=P(A$\cap$B)/P(A) = 0.5
=> P(A)=1/3  P(B)=5/6  P(A$\cup$B)=1/6
$P(A|\bar{B})=P(A)-P(A\cap B)/P(B)$ = 1
No they aren't you can check by def'n or the values you have already.

---
6✅
B: The sum of rolls of 2 dice is at least 10.  B={46,64,55,65,56,66}
A: both the rolls are even A={...}big 
P(A$\cap$B)=3/36 P(B)=6/36
P(A|B)=P(A$\cap$B)/P(B)=1/2

---
7✅
P(A)=3/4  P(B)=1/2  P(A$\cap$B)=3/8=3/4\*1/2 =P(A)P(B) => yes

---
8✅
Law of total probability
$P\left(e\right)=\frac{1}{4}\cdot\frac{1}{6}+\frac{3}{4}\cdot\frac{11}{36}$

---
9✅
Multiplication Rule
$$P\left(e\right)=\frac{\binom{9}{1}\binom{6}{2}}{\binom{15}{3}}\frac{\binom{8}{1}\binom{7}{2}}{\binom{15}{3}}\frac{\binom{7}{1}\binom{8}{2}}{\binom{15}{3}}$$

---
10
$$P(e)=1-\left(2\left(\frac{1}{5}\right)^{2}\left(\frac{4}{5}\right)^{3}+8\ \left(\frac{1}{5}\right)^{3}\left(\frac{4}{5}\right)^{2}+5\left(\frac{1}{5}\right)^{4}\left(\frac{4}{5}\right)^{1}+\left(\frac{1}{5}\right)^{5}\right)$$

---
11
Law of total propability
$$\frac{1}{7}\left(\frac{5}{9}\left(\frac{5}{6}\right)+\frac{4}{9}\left(\frac{4}{6}\right)\right)+\frac{4}{7}\left(\frac{6}{9}\left(\frac{4}{6}\right)+\frac{3}{9}\left(\frac{3}{6}\right)\right)+\frac{2}{7}\left(\frac{7}{9}\left(\frac{3}{6}\right)+\frac{2}{9}\left(\frac{2}{6}\right)\right)$$

---
12✅
Bay's Theorem
R: you get a red 2 times
P(k=0)=25/36   P(k=1)=10/36   P(K=2)=1/36
$$P(k=2|R)=\frac{P(R|k=2)P(k=2)}{\sum_{i=0}^{2}P(R|k=1)P(k=i)}=\frac{2}{7}$$
$$P(k=1|R)=\frac{5}{7}$$
$$P(k=0|R)=0$$

---
13✅
Bay's Theorem
$$\frac{p}{p+\frac{1}{3}\left(1-p\right)}=\frac{2p}{2p-1}$$
for $p=\frac{1}{4}$ than $\frac{1}{2}$

---

14✅
a) Law of total propability
$$\frac{1}{6}\left(\sum_{i=1}^{6}\frac{1}{2^{i}}\ \right)=\frac{21}{128}$$
b) Bay's  Theorem
$$\frac{\frac{1}{6}\left(\frac{1}{2^{6}}\right)}{\frac{1}{6}\left(\sum_{i=1}^{6}\frac{1}{2^{i}}\ \right)}$$

---
15

---
16✅
Bay's  Theorem
FF     TF   TT
1/4   1/2  1/4
0     1/2   1
$$\frac{\frac{1}{4}\cdot1}{\frac{1}{4}0+\frac{1}{2}\frac{1}{2}+\frac{1}{4}\cdot1}$$


